SSA/Core/Framework/Scratch.lean
@@ -1,0 +1,3 @@
+import Lean
+
+#synth GetElem? (Array Lean.Expr) Nat (Lean.Expr) _
