SSA/Projects/SLLVM/Dialect/Refinement.lean
@@ -12,19 +12,26 @@ scoped instance : Refinement (BitVec w) := .ofEq
 @[simp, simp_llvm_split] theorem bv_isRefinedBy_iff (x y : BitVec w) : x ⊑ y ↔ x = y := by rfl
 -- ^^ declare that for pure bitvectors, refinement is just equality
 
-open HRefinement in
-@[simp, simp_denote]
-theorem isRefinedBy_iff (x y : EffectM <| LLVM.IntW w) :
-    x ⊑ y ↔ @IsRefinedBy (StateT _ PoisonOr (PoisonOr _)) (StateT _ PoisonOr (PoisonOr _)) _ x y := by
-  rfl
+-- open HRefinement in
+-- @[simp, simp_denote]
+-- theorem isRefinedBy_iff (x y : EffectM <| LLVM.IntW w) :
+--     x ⊑ y ↔ @IsRefinedBy (StateT _ PoisonOr (PoisonOr _)) (StateT _ PoisonOr (PoisonOr _)) _ x y := by
+--   rfl
 
 instance : DialectHRefinement SLLVM SLLVM where
-  IsRefinedBy := @fun
-    | bitvec v, bitvec w, (x : EffectM <| LLVM.IntW v), (y : EffectM <| LLVM.IntW w) =>
-        ∃ h : v = w, x ⊑ h ▸ y
+  MonadIsRefinedBy := inferInstanceAs <| HRefinement (EffectM _) (EffectM _)
+  IsRefinedBy := @fun (.bitvec <| .concrete v) (.bitvec <| .concrete w) => ⟨
+    fun (x y : LLVM.IntW _) => ∃ h : v = w, x ⊑ h ▸ y
+  ⟩
 
 @[simp, simp_denote]
-theorem dialect_isRefinedBy_iff_of_width_eq (x y : SLLVM.m ⟦bitvec w⟧) :
-    DialectHRefinement.IsRefinedBy x y
-    ↔ HRefinement.IsRefinedBy (α := EffectM <| LLVM.IntW w) (β := EffectM <| LLVM.IntW w) x y := by
-  simp [DialectHRefinement.IsRefinedBy]
+instance instRefinement : DialectHRefinement SLLVM SLLVM where
+  MonadIsRefinedBy := inferInstanceAs <| HRefinement (EffectM _) (EffectM _)
+  IsRefinedBy := @fun (bitvec _) (bitvec _) =>
+    inferInstanceAs <| HRefinement (LLVM.IntW _) (LLVM.IntW _)
+
+-- @[simp, simp_denote]
+-- theorem dialect_isRefinedBy_iff_of_width_eq (x y : SLLVM.m ⟦bitvec w⟧) :
+--     x ⊑ y
+--     ↔ HRefinement.IsRefinedBy (α := EffectM <| LLVM.IntW w) (β := EffectM <| LLVM.IntW w) x y := by
+--   rfl
